adding test examples (atoic functions)

codeTest/test_is_well_chunk_bool.v
@@ -1,5 +1,6 @@
 Require Import ChkPrimitive RelCorrect generated.
-From dx.tests Require Import DxIntegers DxValues DxState DxMonad DxInstructions.
+From dx.tests Require Import DxIntegers DxValues DxMemRegion DxState DxMonad DxInstructions.
+From dx.Type Require Import Bool.
 From dx Require Import ResultMonad IR.
 From Coq Require Import List.
 From compcert Require Import Values Clight Memory.
@@ -7,41 +8,53 @@ Import ListNotations.
 Require Import ZArith.
 
 
+
+Section Is_well_chunk_bool.
+
 (** The program contains our function of interest [fn] *)
 Definition p : Clight.program := prog.
 
 (* [Args,Res] provides the mapping between the Coq and the C types *)
-Definition Args : list CompilableType := [val64CompilableType; val64CompilableType].
-Definition Res : CompilableType := val64CompilableType.
+Definition Args : list CompilableType := [memoryChunkCompilableType].
+Definition Res : CompilableType := boolCompilableType.
 
 (* [f] is a Coq Monadic function with the right type *)
-Definition f : encodeCompilableSymbolType (Some M) (MkCompilableSymbolType Args (Some Res)) := get_addl.
+Definition f : encodeCompilableSymbolType (Some M) (MkCompilableSymbolType Args (Some Res)) := is_well_chunk_bool.
 
 (* [fn] is the Cligth function which has the same behaviour as [f] *)
-Definition fn: Clight.function := f_get_addl.
+Definition fn: Clight.function := f_is_well_chunk_bool.
 
 (* [match_mem] related the Coq monadic state and the C memory *)
-Definition match_mem : stateM -> genv -> Memory.Mem.mem -> Prop :=
+Definition match_mem : stateM -> genv -> Mem.mem -> Prop :=
   fun stm g m =>
     g = globalenv p /\
       (match Globalenvs.Genv.alloc_globals (genv_genv g) (eval_mem stm) global_definitions with
        | None => True
        | Some m' => m' = m
-       end).
+       end)
+.
 
 (* [match_arg] relates the Coq arguments and the C arguments *)
 Definition match_arg_list : DList.t (fun x => coqType x -> Memory.Mem.mem -> val -> Prop) Args :=
-  args_binary_val64_correct.
+  args_block_ptr_correct.
 
 (* [match_res] relates the Coq result and the C result *)
 Definition match_res : coqType Res -> Memory.Mem.mem -> val -> Prop := val64_correct.
 
-Lemma correct_function_addl : correct_function p Args Res f fn match_mem match_arg_list match_res.
+(** How to tell compcert this relation *) (*
+Axiom id_assum: __1004 = IdentDef.mem_region_id.*)
+
+Lemma correct_function_is_well_chunk_bool : correct_function p Args Res f fn match_mem match_arg_list match_res.
 Proof.
   constructor. (*
   - reflexivity.
   - reflexivity.
-  - reflexivity.
+  - unfold Args.
+    simpl.
+    unfold mem_region_type.
+    unfold Clightdefs.tptr.
+    rewrite id_assum.
+    reflexivity.
   - reflexivity.*)
   - unfold Args.
     intro.
@@ -52,16 +65,14 @@ Proof.
     (** Here, we know that v = Val.addl (fst c) (fst c0) and m' = m and the trace is empty*)
     (* We need to do it early or we have problems with existentials *)
     destruct c as (v,v').
-    destruct c0 as (c0,c0').
-    unfold val64_correct in *.
+    unfold block_size_correct in *.
     simpl in H.
-    intuition subst. destruct H3 ; subst.
-    destruct H5 ; subst.
+    intuition subst. clear H2. destruct H1 ; subst.
     simpl.
-    eexists. eexists. eexists.
+    do 3 eexists.
     repeat split.
     (* We need to run the program. Some automation is probably possible *)
-    unfold step1.
+    unfold step2.
     apply Smallstep.plus_star.
     eapply Smallstep.plus_left';eauto.
     econstructor ; eauto.
@@ -75,21 +86,20 @@ Proof.
       reflexivity.
     + simpl.
       unfold Coqlib.list_disjoint.
-      simpl. intuition congruence.
+      simpl; intuition congruence.
     + repeat econstructor; eauto.
     + reflexivity.
-    +  eapply Smallstep.plus_one.
+    + eapply Smallstep.plus_one.
       econstructor; eauto.
-       (* We evaluate the expresssions *)
-      econstructor;eauto.
-      econstructor;eauto.
-      reflexivity.
-      econstructor;eauto.
-      reflexivity.
-      Transparent Archi.ptr64.
-      reflexivity.
-      reflexivity.
-      reflexivity.
-    + unfold match_mem in H0. destruct H0 as [H0 H1]. assumption.
-    + eexists;reflexivity.
+      * econstructor;eauto.
+      * simpl; rewrite <- H1.
+        Transparent Archi.ptr64.
+        reflexivity.
+      * compute; destruct v; simpl in *.
+        eauto.
+    + unfold match_mem in H0.
+      destruct H0; assumption.
+    + eauto.
 Qed.
+
+End Is_well_chunk_bool.
